paxos/proof_helper.dfy
@@ -129,6 +129,24 @@ lemma lemma_ChosenImpliesProposeMsg(c:Constants, ds:DistrSys, b:Ballot, v:Value)
 }
 
 
+
+lemma {:axiom} BallotInductionAxiom1(c:Constants, ds:DistrSys, accpt:Packet, b:Ballot, v:Value) 
+    requires c.WF() && ds.WF(c)
+    requires isAcceptPkt(ds, accpt)
+    requires BalLtEq(b, accpt.msg.bal)
+    requires accpt.msg.bal == b ==>  accpt.msg.val == v
+    requires BalLt(b, accpt.msg.bal) ==> 
+        (exists accpt2:Packet :: 
+            && isAcceptPkt(ds, accpt2) 
+            && BalLtEq(b, accpt2.msg.bal) && BalLt(accpt2.msg.bal, accpt.msg.bal)
+            && accpt2.msg.val == accpt.msg.val)
+    ensures accpt.msg.val == v
+{
+    assume false;
+    // This is axiomatic
+}
+
+
 /*****************************************************************************************
 *                                  Two State Helpers                                     *
 *****************************************************************************************/
@@ -355,7 +373,6 @@ lemma lemma_Set_MinusElem<T>(S:set<T>, e:T, n:int)
     requires e in S
     ensures |S - {e}| == n - 1
 {}
-
 
 /*****************************************************************************************
 *                                        Utils                                           *
